Dom.lean
@@ -54,6 +54,7 @@ import Dom.Mutation.Create
 import Dom.Properties.Create
 import Dom.Validity.Create
 import Dom.Mutation.Clone
+import Dom.Validity.Clone
 import Dom.Properties.Clone
 import Dom.Spec.Remove
 import Dom.Spec.RemoveSound
